
\newcommand{\pwr}{\textsc{pwr}}
\newcommand{\mlt}{\textsc{mlt}}
\newcommand{\fct}{\textsc{fct}}
\newcommand{\fp}{\textsc{fp}}
\newcommand{\Mlt}{\textsc{mlt$^{2}$}}
\newcommand{\Pwr}{\textsc{pwr$^{2}$}}

\newcommand{\fib}{\textsc{fib}}
\newcommand{\Fib}{\textsc{fib$^{2}$}}

\newcommand{\fldp}{\textsc{fld$_{+}$}}
\newcommand{\fldppp}{\textsc{fld$_{+++}$}}
\newcommand{\mn}{\textsc{min}}
\newcommand{\fldm}{\textsc{fld$_{-}$}}
\newcommand{\fldpmm}{\textsc{Pr}}
\newcommand{\fldpmmlia}{\textsc{Pr'}}
\newcommand{\fldpm}{\textsc{fld$_{+/-}$}}
\newcommand{\fldlia}{\textsc{fld$^{\text{LIA}}_{+/-}$}}
\newcommand{\evenp}{\textsc{even$_{+}$}}
\newcommand{\splitev}{\textsc{split}}
\newcommand{\splitfldp}{\textsc{fs}}

\newcommand{\ite}{\mathit{ite}}
\newcommand{\len}{\textsc{len}}
\newcommand{\append}{\textsc{append}}
\newcommand{\cons}{\mathit{cons}}
\newcommand{\nil}{\mathit{nil}}

% Two lengths of the same list
\newcommand{\hornlengthsofsamelist}{
\hcs{
  \begin{aligned}
    \len(xs, a) \gets & xs = \nil, a = 0 \cr
    \len(xs, a) \gets & \len(xs', a') , xs = \cons(x, xs'), a = a' + 1\cr
    \bot \gets & \len(xs, a), \len(xs, b), a \neq b
  \end{aligned}
  }
}

% Fold of the append result

\newcommand{\hornfoldappendedlist}{
\hcs{
  \begin{aligned}
    \fldp(xs, a, a') \gets & xs = \nil, a' = a \cr
    \fldp(xs, a, a') \gets & \fldp(xs', a, a''), xs = \cons(x, xs'), a' = a'' + x \cr
    \append(xs, ys, zs) \gets & xs = \nil, zs = ys \cr
    \append(xs, ys, zs) \gets & \append(xs', ys, zs'), xs = \cons(x, xs'), zs = \cons(x, zs') \cr
    \bot \gets & \fldp(xs, a, a'), \fldp(ys, b, b'), \fldp(zs, c, c'), \append(xs, ys, zs), a = 0, b = 0, c = 0,  a + b \neq c
  \end{aligned}
  }
}

\newcommand{\hornfoldappendedlistfinal}{
\hcs{
  \begin{aligned}
    \fldp(xs, a, a', ys, b, b', zs, c, c') \gets & xs = \nil, ys = \nil, zs = \nil, a' = a, b' = b, c' = c, a = 0, b = 0, c = 0 \cr
    \fldppp(xs, a, a', ys, b, b', zs, c, c') \gets & \fldppp(xs', a, a'', ys', b, b', zs', c, c''), \cr 
        & xs = \nil, a' = a \cr
        & ys = \cons(y, ys'), b' = b'' + y, \cr
        & zs = \cons(x, zs'), c' = c'' + y, \cr
        & a = 0, b = 0, c = 0 \cr
    \fldppp(xs, a, a', ys, b, b', zs, c, c') \gets & \fldppp(xs', a, a'', ys', b, b'', zs', c, c''), \cr 
        & xs = \cons(x, xs'), a' = a'' + x, \cr
        & ys = ys', b' = b'', \cr
        & zs = \cons(x, zs'), c' = c'' + x, \cr
        & a = 0, b = 0, c = 0 \cr
   \bot \gets & \fldppp(xs, a, a', ys, b, b', zs, c, c'), a + b \neq c
  \end{aligned}
  }
}


% Fold over elements on even positions of a list

\newcommand{\hornevenfoldslist}{
\hcs{
  \begin{aligned}
    \fldp(xs, a, a') \gets & xs = \nil, a' = a \cr
    \fldp(xs, a, a') \gets & \fldp(xs', a, a''), xs = \cons(x, xs'), a' = a'' + x \cr
    \splitev(xs, ys, zs) \gets & xs = \nil, ys = \nil, zs = \nil \cr
    \splitev(xs, ys, zs) \gets & xs = \cons(x, \nil), ys = \cons (x, \nil), zs = \nil \cr
    \splitev(xs, ys, zs) \gets & \splitev(xs', ys', zs'), xs = \cons(x, \cons(x', xs')), ys = \cons(x, ys'), zs = \cons(x', zs') \cr
    \bot \gets &  \fldp(xs, a, a'), \fldp(ys, b, b'), \fldp(zs, c, c'), \splitev(xs, ys, zs), a = 0, b = 0, c = 0, a \neq b + c
  \end{aligned}
  }
}

\newcommand{\hornevenfoldslistfinal}{
\hcs{
  \begin{aligned}
    \splitfldp(xs, a, a', ys, b, b', zs, c, c') \gets & xs = \nil, ys = \nil, zs = \nil, a' = a, b' = b, c' = c, a = 0, b = 0, c = 0 \cr
    \splitfldp(xs, a, a', ys, b, b', zs, c, c') \gets & xs = \cons(x, \nil), ys = \cons(x, \nil), zs = \nil, \cr
               & a' = a + x, b' = b + x, c' = c , a = 0, b = 0, c = 0\cr
    \splitfldp(xs, a, a', ys, b, b', zs, c, c') \gets & \splitfldp(xs', a, a'', ys', b, b'', zs', c, c''), \cr
         & xs = \cons(x, \cons(x', xs')), a' = a''' + x, a''' = a'' + x', \cr
         & ys = \cons(x, ys'), b' = b'' + x , \cr
         & zs = \cons(x', zs'),  c' = c'' + x', \cr
         & a = 0, b = 0, c = 0 \cr
    \bot \gets & \splitfldp(xs, a, a', ys, b, b', zs, c, c'), a \neq b
  \end{aligned}
  }
}






